WIP: Closed record types in validator
Some progress on proofs I think

cedar-dafny/validation/types.dfy
@@ -69,7 +69,7 @@ module validation.types {
   }
 
   datatype AttrType = AttrType(ty: Type, isRequired: bool)
-  type RecordType = map<Attr,AttrType>
+  datatype RecordType = RecordType(attrs: map<Attr,AttrType>, is_open: bool)
 
   // Each extension function is associated with argument types, a return type,
   // and an optional method that checks input well-formedness.
