cedar-dafny/validation/thm/model.dfy
@@ -213,20 +213,20 @@ module validation.thm.model {
           }
         }
       case (Record(rt1),Record(rt2),Record(rv)) =>
-        assert forall k | k in rt2 && k in rv :: InstanceOfType(rv[k],rt2[k].ty) by {
-          forall k: Attr | k in rt2 && k in rv
-            ensures InstanceOfType(rv[k],rt2[k].ty)
+        assert forall k | k in rt2.attrs && k in rv :: InstanceOfType(rv[k],rt2.attrs[k].ty) by {
+          forall k: Attr | k in rt2.attrs && k in rv
+            ensures InstanceOfType(rv[k],rt2.attrs[k].ty)
           {
-            assert InstanceOfType(rv[k],rt1[k].ty);
-            assert subtyAttrType(rt1[k],rt2[k]);
-            SubtyCompatMatchPointwise(rt1[k].ty,rt2[k].ty,rv[k]);
+            assert InstanceOfType(rv[k],rt1.attrs[k].ty);
+            assert subtyAttrType(rt1.attrs[k],rt2.attrs[k]);
+            SubtyCompatMatchPointwise(rt1.attrs[k].ty,rt2.attrs[k].ty,rv[k]);
           }
         }
-        assert forall k | k in rt2 && rt2[k].isRequired :: k in rv by {
-          forall k | k in rt2 && rt2[k].isRequired
+        assert forall k | k in rt2.attrs && rt2.attrs[k].isRequired :: k in rv by {
+          forall k | k in rt2.attrs && rt2.attrs[k].isRequired
             ensures k in rv
           {
-            assert subtyAttrType(rt1[k],rt2[k]);
+            assert subtyAttrType(rt1.attrs[k],rt2.attrs[k]);
           }
         }
       case (Entity(e1),Entity(e2),_) =>
@@ -884,7 +884,8 @@ module validation.thm.model {
     // every entry has some type
     requires forall ae :: ae in es ==> ExistsSafeType(r,s,ae.1)
     // and the last instance of every required key is safe at the correct type.
-    requires forall k :: k in rt ==> KeyExists(k,es) && IsSafe(r,s,LastOfKey(k,es),rt[k].ty)
+    requires forall k :: k in rt.attrs ==> KeyExists(k,es) && IsSafe(r,s,LastOfKey(k,es),rt.attrs[k].ty)
+    requires !rt.is_open ==> forall ae :: ae in es ==> ae.0 in rt.attrs.Keys
     ensures IsSafe(r,s,Expr.Record(es),Type.Record(rt))
   {
     reveal IsSafe();
@@ -894,12 +895,12 @@ module validation.thm.model {
       var rv := res.value;
       assert evaluator.interpret(Expr.Record(es)) == base.Ok(Value.Record(rv));
       InterpretRecordLemmaOk(es,r,s);
-      forall k | k in rt
-        ensures InstanceOfType(rv[k],rt[k].ty)
+      forall k | k in rt.attrs
+        ensures InstanceOfType(rv[k],rt.attrs[k].ty)
       {
         var vres := evaluator.interpret(LastOfKey(k,es));
         assert vres == base.Ok(rv[k]);
-        assert InstanceOfType(vres.value,rt[k].ty);
+        assert InstanceOfType(vres.value,rt.attrs[k].ty);
       }
       assert InstanceOfType(Value.Record(rv),Type.Record(rt));
     } else {
@@ -910,7 +911,7 @@ module validation.thm.model {
   lemma ObjectProjSafeRequired(r: Request, s: EntityStore, e: Expr, t: Type, l: Attr, t': AttrType)
     requires IsSafe(r,s,e,t)
     requires t'.isRequired
-    requires SemanticSubty(t,Type.Record(map[l := t']))
+    requires SemanticSubty(t,Type.Record(RecordType(map[l := t'], true)))
     ensures IsSafe(r,s,GetAttr(e,l),t'.ty)
   {
     reveal IsSafe();
@@ -918,7 +919,7 @@ module validation.thm.model {
 
   lemma ObjectProjSafeGetAttrSafe(r: Request, s: EntityStore, e: Expr, t: Type, l: Attr, t': AttrType)
     requires IsSafe(r,s,e,t)
-    requires SemanticSubty(t,Type.Record(map[l := t']))
+    requires SemanticSubty(t,Type.Record(RecordType(map[l := t'], true)))
     requires GetAttrSafe(r,s,e,l)
     ensures IsSafe(r,s,GetAttr(e,l),t'.ty)
   {
@@ -935,7 +936,7 @@ module validation.thm.model {
   }
 
   lemma RecordHasRequiredTrueSafe(r: Request, s: EntityStore, e: Expr, l: Attr, t: AttrType)
-    requires IsSafe(r,s,e,Type.Record(map[l := t]))
+    requires IsSafe(r,s,e,Type.Record(RecordType(map[l := t], true)))
     requires t.isRequired
     ensures IsTrue(r,s,HasAttr(e,l))
   {
@@ -943,10 +944,25 @@ module validation.thm.model {
   }
 
   lemma RecordHasOpenRecSafe(r: Request, s: EntityStore, e: Expr, l: Attr)
-    requires IsSafe(r,s,e,Type.Record(map[]))
+    requires IsSafe(r,s,e,Type.Record(RecordType(map[], true)))
     ensures IsSafe(r,s,HasAttr(e,l),Type.Bool(AnyBool))
   {
     reveal IsSafe();
+  }
+
+  lemma RecordHasClosedRecFalseSafe(r: Request, s: EntityStore, e: Expr, l: Attr, rt: RecordType)
+    requires IsSafe(r,s,e,Type.Record(rt))
+    requires l !in rt.attrs.Keys
+    requires !rt.is_open
+    ensures IsFalse(r,s,HasAttr(e,l))
+  {
+    reveal IsSafe();
+    var evaluator := Evaluator(r,s);
+    var v := evaluator.interpret(e);
+    if v.Ok? {
+      var rv :- assert Value.asRecord(v.value);
+      assert l !in rv.Keys;
+    }
   }
 
   lemma EntityHasImpossibleFalseSafe(r: Request, s: EntityStore, e: Expr, l: Attr, lub: EntityLUB)
